All references of T or U now point to an equivalent τ

TS/StlcProp.lean
@@ -79,18 +79,18 @@ Small-step operational semantics:
 
 Typing:
 ```
-                              Γ x = T₁
+                              Γ x = τ₁
                             ------------                       (var)
-                             Γ ⊢ x ⦂ T₁
+                             Γ ⊢ x ⦂ τ₁
 
-                        x ↦ T₂ ; Γ ⊢ t₁ ⦂ T₁
+                        x ↦ τ₂ ; Γ ⊢ t₁ ⦂ τ₁
                       -------------------------                (abs)
-                       Γ ⊢ λx:T₂. t₁ ⦂ T₂ → T₁
+                       Γ ⊢ λx:τ₂. t₁ ⦂ τ₂ → τ₁
 
-                          Γ ⊢ t₁ ⦂ T₂ → T₁
-                            Γ ⊢ t₂ ⦂ T₂
+                          Γ ⊢ t₁ ⦂ τ₂ → τ₁
+                            Γ ⊢ t₂ ⦂ τ₂
                          ------------------                    (app)
-                           Γ ⊢ t₁ t₂ ⦂ T₁
+                           Γ ⊢ t₁ t₂ ⦂ τ₁
 
                           -----------------                    (tru)
                            Γ ⊢ true ⦂ Bool
@@ -98,9 +98,9 @@ Typing:
                          ------------------                    (fls)
                           Γ ⊢ false ⦂ Bool
 
-             Γ ⊢ t₁ ⦂ Bool    Γ ⊢ t₂ ⦂ T₁    Γ ⊢ t₃ ⦂ T₁
+             Γ ⊢ t₁ ⦂ Bool    Γ ⊢ t₂ ⦂ τ₁    Γ ⊢ t₃ ⦂ τ₁
             ---------------------------------------------      (ite)
-                   Γ ⊢ if t₁ then t₂ else t₃ ⦂ T₁
+                   Γ ⊢ if t₁ then t₂ else t₃ ⦂ τ₁
 ```
 ::::
 
@@ -144,21 +144,21 @@ only well typed but _closed_ — i.e., well typed in the empty
 context.
 
 ```lean
-theorem canonical_forms_bool (t : Tm) (hT : <{ ∅ ⊢ ~t ⦂ Bool }>) (hv : t.IsValue) :
+theorem canonical_forms_bool (t : Tm) (hτ : <{ ∅ ⊢ ~t ⦂ Bool }>) (hv : t.IsValue) :
     t = <{ true }> ∨ t = <{ false }> := by
   cases hv with
-  | abs x τ t₁ => cases hT
+  | abs x τ t₁ => cases hτ
   | tru => left; rfl
   | fls => right; rfl
 
-theorem canonical_forms_fun (t : Tm) (T₁ T₂ : Ty)
-    (hT : <{ ∅ ⊢ ~t ⦂ ~T₁ → ~T₂ }>) (hv : t.IsValue) :
-    ∃ x u, t = <{ λ ~x : ~T₁ . ~u }> := by
+theorem canonical_forms_fun (t : Tm) (τ₁ τ₂ : Ty)
+    (hτ : <{ ∅ ⊢ ~t ⦂ ~τ₁ → ~τ₂ }>) (hv : t.IsValue) :
+    ∃ x u, t = <{ λ ~x : ~τ₁ . ~u }> := by
   cases hv with
-  | abs x τ t₁ => cases hT with | abs _ _ _ _ _ _ =>
+  | abs x τ t₁ => cases hτ with | abs _ _ _ _ _ _ =>
     exists x, t₁
-  | tru => cases hT
-  | fls => cases hT
+  | tru => cases hτ
+  | fls => cases hτ
 ```
 
 # Progress
@@ -188,8 +188,8 @@ _Proof_: By induction on the derivation of `∅ ⊢ t ⦂ τ`.
   is a value.
 
 - If the last rule of the derivation is `HasType.app`, then `t` has the
-  form `t₁ t₂` for some `t₁` and `t₂`, where `∅ ⊢ t₁ ⦂ T₂ → τ`
-  and `∅ ⊢ t₂ ⦂ T₂` for some type `T₂`.  The induction hypothesis
+  form `t₁ t₂` for some `t₁` and `t₂`, where `∅ ⊢ t₁ ⦂ τ₂ → τ`
+  and `∅ ⊢ t₂ ⦂ τ₂` for some type `τ₂`.  The induction hypothesis
   for the first subderivation says that either `t₁` is a value or
   else it can take a reduction step.
 
@@ -216,11 +216,11 @@ _Proof_: By induction on the derivation of `∅ ⊢ t ⦂ τ`.
 ::::
 
 ```lean
-theorem progress (t : Tm) (τ : Ty) (hT : <{ ∅ ⊢ ~t ⦂ ~τ }>) :
+theorem progress (t : Tm) (τ : Ty) (hτ : <{ ∅ ⊢ ~t ⦂ ~τ }>) :
     t.IsValue ∨ ∃ t', t ⟶ t' := by
-  generalize hΓ : (∅ : Context) = Γ at hT
-  induction hT with
-  | var Γ x T₁ h =>
+  generalize hΓ : (∅ : Context) = Γ at hτ
+  induction hτ with
+  | var Γ x τ₁ h =>
     subst hΓ
     -- Contradictory: variables cannot be typed in an empty context.
     rw [PartialMap.getElem_empty] at h
@@ -228,7 +228,7 @@ theorem progress (t : Tm) (τ : Ty) (hT : <{ ∅ ⊢ ~t ⦂ ~τ }>) :
   | abs => left; constructor
   | tru => left; constructor
   | fls => left; constructor
-  | app Γ T₁ T₂ t₁ t₂ h₁ h₂ ih₁ ih₂ =>
+  | app Γ τ₁ τ₂ t₁ t₂ h₁ h₂ ih₁ ih₂ =>
     -- `t = t₁ t₂`.  Proceed by cases on whether `t₁` is a value or steps.
     subst hΓ
     right
@@ -248,7 +248,7 @@ theorem progress (t : Tm) (τ : Ty) (hT : <{ ∅ ⊢ ~t ⦂ ~τ }>) :
       obtain ⟨t₁', h⟩ := hs₁
       exists <{ ~t₁' ~t₂ }>
       constructor <;> assumption
-  | ite Γ t₁ t₂ t₃ T₁ h₁ h₂ h₃ ih₁ ih₂ ih₃ =>
+  | ite Γ t₁ t₂ t₃ τ₁ h₁ h₂ h₃ ih₁ ih₂ ih₃ =>
     subst hΓ
     right
     cases ih₁ rfl with
@@ -276,14 +276,14 @@ Show that progress can also be proved by induction on terms
 instead of induction on typing derivations.
 
 ```lean
-theorem progress' (t : Tm) (τ : Ty) (hT : <{ ∅ ⊢ ~t ⦂ ~τ }>) :
+theorem progress' (t : Tm) (τ : Ty) (hτ : <{ ∅ ⊢ ~t ⦂ ~τ }>) :
     t.IsValue ∨ ∃ t', t ⟶ t' := by
   solution!
     induction t generalizing τ with
     | var x =>
-      cases hT with
+      cases hτ with
       | var _ _ _ h => rw [PartialMap.getElem_empty] at h; cases h
-    | abs x T₂ t₁ _ =>
+    | abs x τ₂ t₁ _ =>
       left
       constructor
     | tru =>
@@ -294,8 +294,8 @@ theorem progress' (t : Tm) (τ : Ty) (hT : <{ ∅ ⊢ ~t ⦂ ~τ }>) :
       constructor
     | app t₁ t₂ ih₁ ih₂ =>
       right
-      cases hT with
-      | app _ _ T₂ _ _ h₁ h₂ =>
+      cases hτ with
+      | app _ _ τ₂ _ _ h₁ h₂ =>
         cases ih₁ _ h₁ with
         | inl hv₁ =>
           obtain ⟨x, u, rfl⟩ := canonical_forms_fun t₁ _ _ h₁ hv₁
@@ -305,7 +305,7 @@ theorem progress' (t : Tm) (τ : Ty) (hT : <{ ∅ ⊢ ~t ⦂ ~τ }>) :
             constructor <;> assumption
           | inr hs₂ =>
             obtain ⟨t₂', h⟩ := hs₂
-            exists <{ (λ ~x : ~T₂ . ~u) ~t₂' }>
+            exists <{ (λ ~x : ~τ₂ . ~u) ~t₂' }>
             apply Step.app2 <;> assumption
         | inr hs₁ =>
           obtain ⟨t₁', h⟩ := hs₁
@@ -314,7 +314,7 @@ theorem progress' (t : Tm) (τ : Ty) (hT : <{ ∅ ⊢ ~t ⦂ ~τ }>) :
           assumption
     | ite t₁ t₂ t₃ ih₁ ih₂ ih₃ =>
       right
-      cases hT with
+      cases hτ with
       | ite _ _ _ _ _ h₁ h₂ h₃ =>
         cases ih₁ _ h₁ with
         | inl hv₁ =>
@@ -497,8 +497,8 @@ preserves types.
 Formally, the so-called _substitution lemma_ says this:
 Suppose we have a term `t` with a free variable `x`, and suppose
 we've assigned a type `τ` to `t` under the assumption that `x` has
-some type `U`.  Also, suppose that we have some other term `v` and
-that we've shown that `v` has type `U`.  Then, since `v` satisfies
+some type `τ'`.  Also, suppose that we have some other term `v` and
+that we've shown that `v` has type `τ'`.  Then, since `v` satisfies
 the assumption we made about `x` when typing `t`, we can
 substitute `v` for each of the occurrences of `x` in `t` and
 obtain a new term that still has type `τ`.
@@ -509,10 +509,10 @@ The _substitution lemma_ says:
 
 - Suppose we have a term `t` with a free variable `x`, and
   suppose we've been able to assign a type `τ` to `t` under the
-  assumption that `x` has some type `U`.
+  assumption that `x` has some type `τ'`.
 
 - Also, suppose that we have some other term `v` and that we've
-  shown that `v` has type `U`.
+  shown that `v` has type `τ'`.
 
 - Then we can substitute `v` for each of the occurrences of
   `x` in `t` and obtain a new term that still has type `τ`.
@@ -522,23 +522,23 @@ The _substitution lemma_ says:
 :::
 
 ```lean
-theorem substitution_preserves_typing (Γ : Context) (x : String) (U : Ty)
+theorem substitution_preserves_typing (Γ : Context) (x : String) (τ' : Ty)
     (t v : Tm) (τ : Ty)
-    (hT : <{ ~x ↦ ~U ; ~Γ ⊢ ~t ⦂ ~τ }>) (hv : <{ ∅ ⊢ ~v ⦂ ~U }>) :
+    (hτ : <{ ~x ↦ ~τ' ; ~Γ ⊢ ~t ⦂ ~τ }>) (hv : <{ ∅ ⊢ ~v ⦂ ~τ' }>) :
     <{ ~Γ ⊢ [~x := ~v] ~t ⦂ ~τ }> := by
-  -- By induction on `t`; in each case we get at the derivation of `hT`.
+  -- By induction on `t`; in each case we get at the derivation of `hτ`.
   induction t generalizing Γ τ with
   | var y =>
-    cases hT with
+    cases hτ with
     | var _ _ _ h =>
       by_cases hxy : x = y
       · subst hxy
         rw [PartialMap.update_eq] at h
         rw [subst_var_eq]
-        have hUT : U = τ := by
+        have hτ'τ : τ' = τ := by
           apply Option.some.inj
           exact h
-        subst hUT
+        subst hτ'τ
         apply weakening_empty
         exact hv
       · rw [PartialMap.update_neq hxy] at h
@@ -546,7 +546,7 @@ theorem substitution_preserves_typing (Γ : Context) (x : String) (U : Ty)
         constructor
         exact h
   | app t₁ t₂ ih₁ ih₂ =>
-    cases hT with
+    cases hτ with
     | app _ _ _ _ _ h₁ h₂ =>
       rw [subst_app]
       constructor
@@ -555,7 +555,7 @@ theorem substitution_preserves_typing (Γ : Context) (x : String) (U : Ty)
       · apply ih₂
         exact h₂
   | abs y S t₁ ih =>
-    cases hT with
+    cases hτ with
     | abs _ _ _ _ _ h =>
       by_cases hxy : x = y
       · subst hxy
@@ -569,17 +569,17 @@ theorem substitution_preserves_typing (Γ : Context) (x : String) (U : Ty)
         apply ih
         exact h
   | tru =>
-    cases hT with
+    cases hτ with
     | tru =>
       rw [subst_tru]
       constructor
   | fls =>
-    cases hT with
+    cases hτ with
     | fls =>
       rw [subst_fls]
       constructor
   | ite c t e ihc iht ihe =>
-    cases hT with
+    cases hτ with
     | ite _ _ _ _ _ h₁ h₂ h₃ =>
       rw [subst_ite]
       constructor
@@ -601,38 +601,38 @@ assign a type to `[x:=v] t`; the result is the same either
 way.
 
 _Proof_: We show, by induction on `t`, that for all `τ` and
-`Γ`, if `x ↦ U ; Γ ⊢ t ⦂ τ` and `∅ ⊢ v ⦂ U`, then
+`Γ`, if `x ↦ τ' ; Γ ⊢ t ⦂ τ` and `∅ ⊢ v ⦂ τ'`, then
 `Γ ⊢ [x:=v]t ⦂ τ`.
 
   - If `t` is a variable there are two cases to consider,
     depending on whether `t` is `x` or some other variable.
 
-      - If `t = x`, then from the fact that `x ↦ U ; Γ ⊢ x ⦂ τ` we conclude that `U = τ`.  We must show that `[x:=v]x = v` has type `τ` under `Γ`, given the assumption that
-        `v` has type `U = τ` under the empty context.  This
+      - If `t = x`, then from the fact that `x ↦ τ' ; Γ ⊢ x ⦂ τ` we conclude that `τ' = τ`.  We must show that `[x:=v]x = v` has type `τ` under `Γ`, given the assumption that
+        `v` has type `τ' = τ` under the empty context.  This
         follows from the weakening lemma.
 
       - If `t` is some variable `y` that is not equal to `x`, then
-        we need only note that `y` has the same type under `x ↦ U ; Γ` as under `Γ`.
+        we need only note that `y` has the same type under `x ↦ τ' ; Γ` as under `Γ`.
 
-  - If `t` is an abstraction `λy:S. t₀`, then `τ = S → T₁` and
-    the IH tells us, for all `Γ'` and `T₀`, that if `x ↦ U ; Γ' ⊢ t₀ ⦂ T₀`, then `Γ' ⊢ [x:=v]t₀ ⦂ T₀`.
+  - If `t` is an abstraction `λy:S. t₀`, then `τ = S → τ₁` and
+    the IH tells us, for all `Γ'` and `τ₀`, that if `x ↦ τ' ; Γ' ⊢ t₀ ⦂ τ₀`, then `Γ' ⊢ [x:=v]t₀ ⦂ τ₀`.
     Moreover, by inspecting the typing rules we see it must be
-    the case that `y ↦ S ; x ↦ U ; Γ ⊢ t₀ ⦂ T₁`.
+    the case that `y ↦ S ; x ↦ τ' ; Γ ⊢ t₀ ⦂ τ₁`.
 
     The substitution in the conclusion behaves differently
     depending on whether `x` and `y` are the same variable.
 
     First, suppose `x = y`.  Then, by the definition of
-    substitution, `[x:=v]t = t`, so we just need to show `Γ ⊢ t ⦂ τ`.  Using `HasType.abs`, we need to show that `y ↦ S ; Γ ⊢ t₀ ⦂ T₁`. But we know `y ↦ S ; x ↦ U ; Γ ⊢ t₀ ⦂ T₁`,
+    substitution, `[x:=v]t = t`, so we just need to show `Γ ⊢ t ⦂ τ`.  Using `HasType.abs`, we need to show that `y ↦ S ; Γ ⊢ t₀ ⦂ τ₁`. But we know `y ↦ S ; x ↦ τ' ; Γ ⊢ t₀ ⦂ τ₁`,
     and the claim follows since `x = y`.
 
     Second, suppose `x ≠ y`. Again, using `HasType.abs`,
-    we need to show that `y ↦ S ; Γ ⊢ [x:=v]t₀ ⦂ T₁`.
+    we need to show that `y ↦ S ; Γ ⊢ [x:=v]t₀ ⦂ τ₁`.
     Since `x ≠ y`, we have
-    `y ↦ S ; x ↦ U ; Γ = x ↦ U ; y ↦ S ; Γ`. So
-    we have `x ↦ U ; y ↦ S ; Γ ⊢ t₀ ⦂ T₁`. Then, the
+    `y ↦ S ; x ↦ τ' ; Γ = x ↦ τ' ; y ↦ S ; Γ`. So
+    we have `x ↦ τ' ; y ↦ S ; Γ ⊢ t₀ ⦂ τ₁`. Then, the
     IH applies (taking `Γ' = y ↦ S ; Γ`), giving us
-    `y ↦ S ; Γ ⊢ [x:=v]t₀ ⦂ T₁`, as required.
+    `y ↦ S ; Γ ⊢ [x:=v]t₀ ⦂ τ₁`, as required.
 
   - If `t` is an application `t₁ t₂`, the result follows
     straightforwardly from the definition of substitution and the
@@ -643,7 +643,7 @@ _Proof_: We show, by induction on `t`, that for all `τ` and
 
 ::::full
 One technical subtlety in the statement of the above lemma is that
-we assume `v` has type `U` in the _empty_ context — in other
+we assume `v` has type `τ'` in the _empty_ context — in other
 words, we assume `v` is closed.  (Since we are using a simple
 definition of substitution that is not capture-avoiding, it doesn't
 make sense to substitute non-closed terms into other terms.
@@ -658,23 +658,23 @@ proved by induction on typing derivations instead
 of induction on terms.
 
 ```lean
-theorem substitution_preserves_typing_from_typing_ind (Γ : Context) (x : String) (U : Ty)
+theorem substitution_preserves_typing_from_typing_ind (Γ : Context) (x : String) (τ' : Ty)
     (t v : Tm) (τ : Ty)
-    (hT : <{ ~x ↦ ~U ; ~Γ ⊢ ~t ⦂ ~τ }>) (hv : <{ ∅ ⊢ ~v ⦂ ~U }>) :
+    (hτ : <{ ~x ↦ ~τ' ; ~Γ ⊢ ~t ⦂ ~τ }>) (hv : <{ ∅ ⊢ ~v ⦂ ~τ' }>) :
     <{ ~Γ ⊢ [~x := ~v] ~t ⦂ ~τ }> := by
   solution!
-    generalize hΓ : (x →ₚ U ; Γ) = Γ₀ at hT
-    induction hT generalizing Γ with
-    | var _ y T₁ h =>
+    generalize hΓ : (x →ₚ τ' ; Γ) = Γ₀ at hτ
+    induction hτ generalizing Γ with
+    | var _ y τ₁ h =>
       subst hΓ
       by_cases hxy : x = y
       · subst hxy
         rw [PartialMap.update_eq] at h
         rw [subst_var_eq]
-        have hUT : U = T₁ := by
+        have hτ'τ : τ' = τ₁ := by
           apply Option.some.inj
           exact h
-        subst hUT
+        subst hτ'τ
         apply weakening_empty
         exact hv
       · rw [PartialMap.update_neq hxy] at h
@@ -732,14 +732,14 @@ the small-step reduction relation preserves types.
 
 ```lean
 theorem preservation (t t' : Tm) (τ : Ty)
-    (hT : <{ ∅ ⊢ ~t ⦂ ~τ }>) (hs : t ⟶ t') : <{ ∅ ⊢ ~t' ⦂ ~τ }> := by
-  generalize hΓ : (∅ : Context) = Γ at hT
-  induction hT generalizing t' with
+    (hτ : <{ ∅ ⊢ ~t ⦂ ~τ }>) (hs : t ⟶ t') : <{ ∅ ⊢ ~t' ⦂ ~τ }> := by
+  generalize hΓ : (∅ : Context) = Γ at hτ
+  induction hτ generalizing t' with
   | var => cases hs
   | abs => cases hs
   | tru => cases hs
   | fls => cases hs
-  | app Γ T₁ T₂ t₁ t₂ h₁ h₂ ih₁ ih₂ =>
+  | app Γ τ₁ τ₂ t₁ t₂ h₁ h₂ ih₁ ih₂ =>
     subst hΓ
     cases hs with
     | appAbs _ _ _ _ _ =>
@@ -761,7 +761,7 @@ theorem preservation (t t' : Tm) (τ : Ty)
       · apply ih₂
         · exact h
         · rfl
-  | ite Γ t₁ t₂ t₃ T₁ h₁ h₂ h₃ ih₁ ih₂ ih₃ =>
+  | ite Γ t₁ t₂ t₃ τ₁ h₁ h₂ h₃ ih₁ ih₂ ih₃ =>
     subst hΓ
     cases hs with
     | ifTrue => exact h₂
@@ -783,24 +783,24 @@ _Proof_: By induction on the derivation of `∅ ⊢ t ⦂ τ`.
   cases `t` cannot take a step.
 
 - If the last rule in the derivation is `HasType.app`, then `t = t₁ t₂`,
-  and there are subderivations showing that `∅ ⊢ t₁ ⦂ T₂ → τ` and
-  `∅ ⊢ t₂ ⦂ T₂` plus two induction hypotheses: (1) `t₁ ⟶ t₁'`
-  implies `∅ ⊢ t₁' ⦂ T₂ → τ` and (2) `t₂ ⟶ t₂'` implies `∅ ⊢ t₂' ⦂ T₂`.  There are now three subcases to consider, one for
+  and there are subderivations showing that `∅ ⊢ t₁ ⦂ τ₂ → τ` and
+  `∅ ⊢ t₂ ⦂ τ₂` plus two induction hypotheses: (1) `t₁ ⟶ t₁'`
+  implies `∅ ⊢ t₁' ⦂ τ₂ → τ` and (2) `t₂ ⟶ t₂'` implies `∅ ⊢ t₂' ⦂ τ₂`.  There are now three subcases to consider, one for
   each rule that could be used to show that `t₁ t₂` takes a step
   to `t'`.
 
     - If `t₁ t₂` takes a step by `Step.app1`, with `t₁` stepping to
       `t₁'`, then, by the first IH, `t₁'` has the same type as
-      `t₁` (`∅ ⊢ t₁' ⦂ T₂ → τ`), and hence by `HasType.app` `t₁' t₂` has
+      `t₁` (`∅ ⊢ t₁' ⦂ τ₂ → τ`), and hence by `HasType.app` `t₁' t₂` has
       type `τ`.
 
     - The `Step.app2` case is similar, using the second IH.
 
-    - If `t₁ t₂` takes a step by `Step.appAbs`, then `t₁ = λx:T₀. t₀` and `t₁ t₂` steps to `[x:=t₂]t₀`; the desired
+    - If `t₁ t₂` takes a step by `Step.appAbs`, then `t₁ = λx:τ₀. t₀` and `t₁ t₂` steps to `[x:=t₂]t₀`; the desired
       result now follows from the substitution lemma.
 
-- If the last rule in the derivation is `HasType.ite`, then `t = if t₁ then t₂ else t₃`, with `∅ ⊢ t₁ ⦂ Bool`, `∅ ⊢ t₂ ⦂ T₁`, and
-  `∅ ⊢ t₃ ⦂ T₁`, and with three induction hypotheses: (1) `t₁ ⟶ t₁'` implies `∅ ⊢ t₁' ⦂ Bool`, (2) `t₂ ⟶ t₂'` implies `∅ ⊢ t₂' ⦂ T₁`, and (3) `t₃ ⟶ t₃'` implies `∅ ⊢ t₃' ⦂ T₁`.
+- If the last rule in the derivation is `HasType.ite`, then `t = if t₁ then t₂ else t₃`, with `∅ ⊢ t₁ ⦂ Bool`, `∅ ⊢ t₂ ⦂ τ₁`, and
+  `∅ ⊢ t₃ ⦂ τ₁`, and with three induction hypotheses: (1) `t₁ ⟶ t₁'` implies `∅ ⊢ t₁' ⦂ Bool`, (2) `t₂ ⟶ t₂'` implies `∅ ⊢ t₂' ⦂ τ₁`, and (3) `t₃ ⟶ t₃'` implies `∅ ⊢ t₃' ⦂ τ₁`.
 
   There are again three subcases to consider, depending on how `t`
   steps.
@@ -859,7 +859,7 @@ Alternative formulation.
 theorem not_subject_expansion_alt :
     ¬ (∀ (t t' : Tm) (τ : Ty), t ⟶ t' ∧ <{ ∅ ⊢ ~t' ⦂ ~τ }> → <{ ∅ ⊢ ~t ⦂ ~τ }>) := by
   intro hse
-  have hT : <{ ∅ ⊢ (λ x : Bool → Bool . λ y : Bool . y) true ⦂ Bool → Bool }> := by
+  have hτ : <{ ∅ ⊢ (λ x : Bool → Bool . λ y : Bool . y) true ⦂ Bool → Bool }> := by
     apply hse _ <{ λ y : Bool . y }>
     constructor
     · apply Step.appAbs
@@ -867,7 +867,7 @@ theorem not_subject_expansion_alt :
     · apply HasType.abs
       apply HasType.var
       rfl
-  cases hT with
+  cases hτ with
   | app _ _ _ _ _ h₁ h₂ =>
     cases h₁ with
     | abs _ _ _ _ _ _ =>
@@ -896,20 +896,20 @@ term can _never_ reach a stuck state.
 def Tm.IsStuck (t : Tm) : Prop := IsNormalForm Step t ∧ ¬ t.IsValue
 
 theorem type_soundness (t t' : Tm) (τ : Ty)
-    (hT : <{ ∅ ⊢ ~t ⦂ ~τ }>) (hm : t ⟶* t') : ¬ t'.IsStuck := by
+    (hτ : <{ ∅ ⊢ ~t ⦂ ~τ }>) (hm : t ⟶* t') : ¬ t'.IsStuck := by
   intro hst
   obtain ⟨hnf, hnv⟩ := hst
   induction hm with
   | refl u =>
     solution!
-      cases progress u τ hT with
+      cases progress u τ hτ with
       | inl hv => exact hnv hv
       | inr hs => exact hnf hs
   | step u w z h₁ _ ih =>
     solution!
       apply ih
       · apply preservation
-        · exact hT
+        · exact hτ
         · exact h₁
       · exact hnf
       · exact hnv
@@ -929,19 +929,19 @@ Another nice property of the STLC is that types are unique: a
 given term (in a given context) has at most one type.
 
 ```lean
-theorem unique_types (Γ : Context) (e : Tm) (τ T' : Ty)
-    (h : <{ ~Γ ⊢ ~e ⦂ ~τ }>) (h' : <{ ~Γ ⊢ ~e ⦂ ~T' }>) : τ = T' := by
+theorem unique_types (Γ : Context) (e : Tm) (τ τ' : Ty)
+    (h : <{ ~Γ ⊢ ~e ⦂ ~τ }>) (h' : <{ ~Γ ⊢ ~e ⦂ ~τ' }>) : τ = τ' := by
   solution!
-    induction h generalizing T' with
+    induction h generalizing τ' with
     | var _ _ _ hx =>
       cases h' with
       | var _ _ _ hx' =>
         rw [hx] at hx'
         injection hx'
-    | abs _ _ T₁ _ _ _ ih =>
+    | abs _ _ τ₁ _ _ _ ih =>
       cases h' with
-      | abs _ _ T₁' _ _ hb' =>
-        have heq : T₁ = T₁' := by
+      | abs _ _ τ₁' _ _ hb' =>
+        have heq : τ₁ = τ₁' := by
           apply ih
           exact hb'
         rw [heq]
@@ -989,9 +989,9 @@ of the same name.
 More technically, a variable `x` _appears free in_ a term `t` if
 `t` contains some occurrence of `x` that is not under an
 abstraction labeled `x`. For example:
-  - `y` appears free, but `x` does not, in `λx:τ → U. x y`
-  - both `x` and `y` appear free in `(λx:τ → U. x y) x`
-  - no variables appear free in `λx:τ → U. λy:τ. x y`
+  - `y` appears free, but `x` does not, in `λx:τ → τ'. x y`
+  - both `x` and `y` appear free in `(λx:τ → τ'. x y) x`
+  - no variables appear free in `λx:τ → τ'. λy:τ. x y`
 
 We write this `x ∈ᶠ t`, reading the relation as "`x` is one of the free
 variables of `t`".  Formally:
@@ -1005,8 +1005,8 @@ inductive AppearsFreeIn (x : String) : Tm → Prop where
   | var : x ∈ᶠ (Tm.var x)
   | app1 (t₁ t₂ : Tm) (h : x ∈ᶠ t₁) : x ∈ᶠ <{ ~t₁ ~t₂ }>
   | app2 (t₁ t₂ : Tm) (h : x ∈ᶠ t₂) : x ∈ᶠ <{ ~t₁ ~t₂ }>
-  | abs (y : String) (T₁ : Ty) (t₁ : Tm) (hne : y ≠ x) (h : x ∈ᶠ t₁) :
-      x ∈ᶠ <{ λ ~y : ~T₁ . ~t₁ }>
+  | abs (y : String) (τ₁ : Ty) (t₁ : Tm) (hne : y ≠ x) (h : x ∈ᶠ t₁) :
+      x ∈ᶠ <{ λ ~y : ~τ₁ . ~t₁ }>
   | ite1 (t₁ t₂ t₃ : Tm) (h : x ∈ᶠ t₁) : x ∈ᶠ <{ if ~t₁ then ~t₂ else ~t₃ }>
   | ite2 (t₁ t₂ t₃ : Tm) (h : x ∈ᶠ t₂) : x ∈ᶠ <{ if ~t₁ then ~t₂ else ~t₃ }>
   | ite3 (t₁ t₂ t₃ : Tm) (h : x ∈ᶠ t₃) : x ∈ᶠ <{ if ~t₁ then ~t₂ else ~t₃ }>
@@ -1073,12 +1073,12 @@ in `t`, that, for all contexts `Γ`, if `t` is well typed under
   `Γ` as well, and the IH gives us exactly the conclusion we
   want.
 
-- The only remaining case is `AppearsFreeIn.abs`.  In this case `t = λy:T₁. t₁` and `x` appears free in `t₁`, and we also know that
+- The only remaining case is `AppearsFreeIn.abs`.  In this case `t = λy:τ₁. t₁` and `x` appears free in `t₁`, and we also know that
   `x` is different from `y`.  The difference from the previous
   cases is that, whereas `t` is well typed under `Γ`, its body
-  `t₁` is well typed under `y ↦ T₁ ; Γ`, so the IH allows us
+  `t₁` is well typed under `y ↦ τ₁ ; Γ`, so the IH allows us
   to conclude that `x` is assigned some type by the extended
-  context `y ↦ T₁ ; Γ`.  To conclude that `Γ` assigns a
+  context `y ↦ τ₁ ; Γ`.  To conclude that `Γ` assigns a
   type to `x`, we appeal to lemma `PartialMap.update_neq`, noting that `x`
   and `y` are different variables.
 
@@ -1087,42 +1087,42 @@ Complete the following proof.
 
 ```lean
 theorem free_in_context (x : String) (t : Tm) (τ : Ty) (Γ : Context)
-    (ha : x ∈ᶠ t) (hT : <{ ~Γ ⊢ ~t ⦂ ~τ }>) : ∃ T', Γ[x] = some T' := by
+    (ha : x ∈ᶠ t) (hτ : <{ ~Γ ⊢ ~t ⦂ ~τ }>) : ∃ τ', Γ[x] = some τ' := by
   induction ha generalizing Γ τ with
   | var =>
-    cases hT with
+    cases hτ with
     | var _ _ _ h =>
       constructor
       exact h
   | app1 _ _ _ ih =>
-    cases hT with
+    cases hτ with
     | app _ _ _ _ _ h₁ _ =>
       apply ih
       exact h₁
   | app2 _ _ _ ih =>
-    cases hT with
+    cases hτ with
     | app _ _ _ _ _ _ h₂ =>
       apply ih
       exact h₂
   | abs y _ _ hne _ ih =>
     solution!
-      cases hT with
+      cases hτ with
       | abs _ _ _ _ _ hb =>
-        obtain ⟨T', h⟩ := ih _ _ hb
+        obtain ⟨τ', h⟩ := ih _ _ hb
         rw [PartialMap.update_neq hne] at h
-        exists T'
+        exists τ'
   | ite1 _ _ _ _ ih =>
-    cases hT with
+    cases hτ with
     | ite _ _ _ _ _ h₁ _ _ =>
       apply ih
       exact h₁
   | ite2 _ _ _ _ ih =>
-    cases hT with
+    cases hτ with
     | ite _ _ _ _ _ _ h₂ _ =>
       apply ih
       exact h₂
   | ite3 _ _ _ _ ih =>
-    cases hT with
+    cases hτ with
     | ite _ _ _ _ _ _ _ h₃ =>
       apply ih
       exact h₃
@@ -1135,10 +1135,10 @@ no free variables).
 
 :::::exercise (rating := 2) (name := "typable_empty_closed") (optional := true)
 ```lean
-theorem typable_empty_closed (t : Tm) (τ : Ty) (hT : <{ ∅ ⊢ ~t ⦂ ~τ }>) : t.Closed := by
+theorem typable_empty_closed (t : Tm) (τ : Ty) (hτ : <{ ∅ ⊢ ~t ⦂ ~τ }>) : t.Closed := by
   solution!
     intro x ha
-    obtain ⟨T', hc⟩ := free_in_context x t τ ∅ ha hT
+    obtain ⟨τ', hc⟩ := free_in_context x t τ ∅ ha hτ
     rw [PartialMap.getElem_empty] at hc
     cases hc
 ```
@@ -1158,27 +1158,27 @@ _Proof_: By induction on the derivation of `Γ ⊢ t ⦂ τ`.
   `Γ x = τ`.  By assumption, `Γ' x = τ` as well, and hence
   `Γ' ⊢ t ⦂ τ` by `HasType.var`.
 
-- If the last rule was `HasType.abs`, then `t = λy:T₂. t₁`, with `τ = T₂ → T₁` and `y ↦ T₂ ; Γ ⊢ t₁ ⦂ T₁`.  The induction
-  hypothesis states that for any context `Γ''`, if `y ↦ T₂ ; Γ` and `Γ''` assign the same types to all the free
-  variables in `t₁`, then `t₁` has type `T₁` under `Γ''`.
+- If the last rule was `HasType.abs`, then `t = λy:τ₂. t₁`, with `τ = τ₂ → τ₁` and `y ↦ τ₂ ; Γ ⊢ t₁ ⦂ τ₁`.  The induction
+  hypothesis states that for any context `Γ''`, if `y ↦ τ₂ ; Γ` and `Γ''` assign the same types to all the free
+  variables in `t₁`, then `t₁` has type `τ₁` under `Γ''`.
   Let `Γ'` be a context which agrees with `Γ` on the free
-  variables in `t`; we must show `Γ' ⊢ λy:T₂. t₁ ⦂ T₂ → T₁`.
+  variables in `t`; we must show `Γ' ⊢ λy:τ₂. t₁ ⦂ τ₂ → τ₁`.
 
-  By `HasType.abs`, it suffices to show that `y ↦ T₂ ; Γ' ⊢ t₁ ⦂ T₁`.  By the IH (setting `Γ'' = y ↦ T₂ ; Γ'`), it
-  suffices to show that `y ↦ T₂ ; Γ` and `y ↦ T₂ ; Γ'` agree
+  By `HasType.abs`, it suffices to show that `y ↦ τ₂ ; Γ' ⊢ t₁ ⦂ τ₁`.  By the IH (setting `Γ'' = y ↦ τ₂ ; Γ'`), it
+  suffices to show that `y ↦ τ₂ ; Γ` and `y ↦ τ₂ ; Γ'` agree
   on all the variables that appear free in `t₁`.
 
   Any variable occurring free in `t₁` must be either `y` or some
-  other variable.  `y ↦ T₂ ; Γ` and `y ↦ T₂ ; Γ'` clearly
+  other variable.  `y ↦ τ₂ ; Γ` and `y ↦ τ₂ ; Γ'` clearly
   agree on `y`.  Otherwise, note that any variable other than `y`
-  that occurs free in `t₁` also occurs free in `t = λy:T₂. t₁`,
+  that occurs free in `t₁` also occurs free in `t = λy:τ₂. t₁`,
   and by assumption `Γ` and `Γ'` agree on all such
-  variables; hence so do `y ↦ T₂ ; Γ` and `y ↦ T₂ ; Γ'`.
+  variables; hence so do `y ↦ τ₂ ; Γ` and `y ↦ τ₂ ; Γ'`.
 
-- If the last rule was `HasType.app`, then `t = t₁ t₂`, with `Γ ⊢ t₁ ⦂ T₂ → τ` and `Γ ⊢ t₂ ⦂ T₂`.  One induction
+- If the last rule was `HasType.app`, then `t = t₁ t₂`, with `Γ ⊢ t₁ ⦂ τ₂ → τ` and `Γ ⊢ t₂ ⦂ τ₂`.  One induction
   hypothesis states that for all contexts `Γ'`, if `Γ'`
   agrees with `Γ` on the free variables in `t₁`, then `t₁` has
-  type `T₂ → τ` under `Γ'`; there is a similar IH for `t₂`.
+  type `τ₂ → τ` under `Γ'`; there is a similar IH for `t₂`.
   We must show that `t₁ t₂` also has type `τ` under `Γ'`,
   given the assumption that `Γ'` agrees with `Γ` on all
   the free variables in `t₁ t₂`.  By `HasType.app`, it suffices to show
@@ -1192,9 +1192,9 @@ Complete the following proof.
 
 ```lean
 theorem context_invariance (Γ Γ' : Context) (t : Tm) (τ : Ty)
-    (hT : <{ ~Γ ⊢ ~t ⦂ ~τ }>) (hf : ∀ x, x ∈ᶠ t → Γ[x] = Γ'[x]) :
+    (hτ : <{ ~Γ ⊢ ~t ⦂ ~τ }>) (hf : ∀ x, x ∈ᶠ t → Γ[x] = Γ'[x]) :
     <{ ~Γ' ⊢ ~t ⦂ ~τ }> := by
-  induction hT generalizing Γ' with
+  induction hτ generalizing Γ' with
   | var _ x _ h =>
     solution!
       constructor
@@ -1288,12 +1288,12 @@ theorem preservation_statement :
 See `progress` and `preservation` above.  Their statements are:
 
 ```
-theorem progress_statement (t : Tm) (τ : Ty) (hT : <{ ∅ ⊢ ~t ⦂ ~τ }>) :
+theorem progress_statement (t : Tm) (τ : Ty) (hτ : <{ ∅ ⊢ ~t ⦂ ~τ }>) :
     t.IsValue ∨ ∃ t', t ⟶ t' := by
   sorry
 
 theorem preservation_statement (t t' : Tm) (τ : Ty)
-    (hT : <{ ∅ ⊢ ~t ⦂ ~τ }>) (hs : t ⟶ t') : <{ ∅ ⊢ ~t' ⦂ ~τ }> := by
+    (hτ : <{ ∅ ⊢ ~t ⦂ ~τ }>) (hs : t ⟶ t') : <{ ∅ ⊢ ~t' ⦂ ~τ }> := by
   sorry
 ```
 :::
@@ -1589,19 +1589,19 @@ and a proof that progress then fails.
 namespace StlcVar1
 
 inductive HasType : Context → Tm → Ty → Prop where
-  | var (Γ : Context) (x : String) (T₁ : Ty) (h : Γ[x] = some T₁) :
-      HasType Γ (.var x) T₁
-  | abs (Γ : Context) (x : String) (T₁ T₂ : Ty) (t₁ : Tm)
-      (h : HasType (x →ₚ T₂ ; Γ) t₁ T₁) :
-      HasType Γ <{ λ ~x : ~T₂ . ~t₁ }> <{ ~T₂ → ~T₁ }>
-  | app (Γ : Context) (T₁ T₂ : Ty) (t₁ t₂ : Tm)
-      (h₁ : HasType Γ t₁ <{ ~T₂ → ~T₁ }>) (h₂ : HasType Γ t₂ T₂) :
-      HasType Γ <{ ~t₁ ~t₂ }> T₁
+  | var (Γ : Context) (x : String) (τ₁ : Ty) (h : Γ[x] = some τ₁) :
+      HasType Γ (.var x) τ₁
+  | abs (Γ : Context) (x : String) (τ₁ τ₂ : Ty) (t₁ : Tm)
+      (h : HasType (x →ₚ τ₂ ; Γ) t₁ τ₁) :
+      HasType Γ <{ λ ~x : ~τ₂ . ~t₁ }> <{ ~τ₂ → ~τ₁ }>
+  | app (Γ : Context) (τ₁ τ₂ : Ty) (t₁ t₂ : Tm)
+      (h₁ : HasType Γ t₁ <{ ~τ₂ → ~τ₁ }>) (h₂ : HasType Γ t₂ τ₂) :
+      HasType Γ <{ ~t₁ ~t₂ }> τ₁
   | tru (Γ : Context) : HasType Γ <{ true }> <{ Bool }>
   | fls (Γ : Context) : HasType Γ <{ false }> <{ Bool }>
-  | ite (Γ : Context) (t₁ t₂ t₃ : Tm) (T₁ : Ty)
-      (h₁ : HasType Γ t₁ <{ Bool }>) (h₂ : HasType Γ t₂ T₁) (h₃ : HasType Γ t₃ T₁) :
-      HasType Γ <{ if ~t₁ then ~t₂ else ~t₃ }> T₁
+  | ite (Γ : Context) (t₁ t₂ t₃ : Tm) (τ₁ : Ty)
+      (h₁ : HasType Γ t₁ <{ Bool }>) (h₂ : HasType Γ t₂ τ₁) (h₃ : HasType Γ t₃ τ₁) :
+      HasType Γ <{ if ~t₁ then ~t₂ else ~t₃ }> τ₁
   | funnyAbs (x : String) (t₁ : Tm) :
       HasType ∅ <{ λ ~x : Bool . ~t₁ }> <{ Bool }>
 
@@ -1664,7 +1664,7 @@ booleans, for brevity).
 
 ```lean
 inductive Ty where
-  | arrow (T₁ T₂ : Ty)
+  | arrow (τ₁ τ₂ : Ty)
   | nat
 ```
 
@@ -1718,8 +1718,8 @@ scoped macro_rules (kind := Stlc.tyBracket)
       match x.getId.toString with
       | "Nat" => `(Ty.nat)
       | _ => `(($x : Ty))
-  | `(<{ $T₁:stlcTy → $T₂:stlcTy }>)  => `(Ty.arrow <{ $T₁:stlcTy }> <{ $T₂:stlcTy }>)
-  | `(<{ $T₁:stlcTy -> $T₂:stlcTy }>) => `(Ty.arrow <{ $T₁:stlcTy }> <{ $T₂:stlcTy }>)
+  | `(<{ $τ₁:stlcTy → $τ₂:stlcTy }>)  => `(Ty.arrow <{ $τ₁:stlcTy }> <{ $τ₂:stlcTy }>)
+  | `(<{ $τ₁:stlcTy -> $τ₂:stlcTy }>) => `(Ty.arrow <{ $τ₁:stlcTy }> <{ $τ₂:stlcTy }>)
 ```
 ::::
 
@@ -2032,7 +2032,7 @@ Next, the values.
 inductive Tm.IsValue : Tm → Prop where
 -- SOLUTION
   -- In the pure STLC, function abstractions were the only values:
-  | abs (x : String) (T₂ : Ty) (t₁ : Tm) : Tm.IsValue <{ λ ~x : ~T₂ . ~t₁ }>
+  | abs (x : String) (τ₂ : Ty) (t₁ : Tm) : Tm.IsValue <{ λ ~x : ~τ₂ . ~t₁ }>
   -- now the numbers are values too.
   | const (n : Nat) : Tm.IsValue (.const n)
 -- END SOLUTION
@@ -2152,14 +2152,14 @@ Now the typing relation.
 inductive HasType : Context → Tm → Ty → Prop where
 -- SOLUTION
   -- The typing rules for variables, abstraction, and application are from STLC.
-  | var (Γ : Context) (x : String) (T₁ : Ty) (h : Γ[x] = some T₁) :
-      <{ ~Γ ⊢ ~(Tm.var x) ⦂ ~T₁ }>
-  | abs (Γ : Context) (x : String) (T₁ T₂ : Ty) (t₁ : Tm)
-      (h : <{ ~x ↦ ~T₂ ; ~Γ ⊢ ~t₁ ⦂ ~T₁ }>) :
-      <{ ~Γ ⊢ λ ~x : ~T₂ . ~t₁ ⦂ ~T₂ → ~T₁ }>
-  | app (Γ : Context) (T₁ T₂ : Ty) (t₁ t₂ : Tm)
-      (h₁ : <{ ~Γ ⊢ ~t₁ ⦂ ~T₂ → ~T₁ }>) (h₂ : <{ ~Γ ⊢ ~t₂ ⦂ ~T₂ }>) :
-      <{ ~Γ ⊢ ~t₁ ~t₂ ⦂ ~T₁ }>
+  | var (Γ : Context) (x : String) (τ₁ : Ty) (h : Γ[x] = some τ₁) :
+      <{ ~Γ ⊢ ~(Tm.var x) ⦂ ~τ₁ }>
+  | abs (Γ : Context) (x : String) (τ₁ τ₂ : Ty) (t₁ : Tm)
+      (h : <{ ~x ↦ ~τ₂ ; ~Γ ⊢ ~t₁ ⦂ ~τ₁ }>) :
+      <{ ~Γ ⊢ λ ~x : ~τ₂ . ~t₁ ⦂ ~τ₂ → ~τ₁ }>
+  | app (Γ : Context) (τ₁ τ₂ : Ty) (t₁ t₂ : Tm)
+      (h₁ : <{ ~Γ ⊢ ~t₁ ⦂ ~τ₂ → ~τ₁ }>) (h₂ : <{ ~Γ ⊢ ~t₂ ⦂ ~τ₂ }>) :
+      <{ ~Γ ⊢ ~t₁ ~t₂ ⦂ ~τ₁ }>
   -- The remaining five are the typing rules for arithmetic expressions.
   | const (Γ : Context) (n : Nat) :
       <{ ~Γ ⊢ ~(Tm.const n) ⦂ Nat }>
@@ -2170,10 +2170,10 @@ inductive HasType : Context → Tm → Ty → Prop where
   | mult (Γ : Context) (t₁ t₂ : Tm)
       (h₁ : <{ ~Γ ⊢ ~t₁ ⦂ Nat }>) (h₂ : <{ ~Γ ⊢ ~t₂ ⦂ Nat }>) :
       <{ ~Γ ⊢ ~t₁ * ~t₂ ⦂ Nat }>
-  | ite0 (Γ : Context) (t₁ t₂ t₃ : Tm) (T₀ : Ty)
-      (h₁ : <{ ~Γ ⊢ ~t₁ ⦂ Nat }>) (h₂ : <{ ~Γ ⊢ ~t₂ ⦂ ~T₀ }>)
-      (h₃ : <{ ~Γ ⊢ ~t₃ ⦂ ~T₀ }>) :
-      <{ ~Γ ⊢ if0 ~t₁ then ~t₂ else ~t₃ ⦂ ~T₀ }>
+  | ite0 (Γ : Context) (t₁ t₂ t₃ : Tm) (τ₀ : Ty)
+      (h₁ : <{ ~Γ ⊢ ~t₁ ⦂ Nat }>) (h₂ : <{ ~Γ ⊢ ~t₂ ⦂ ~τ₀ }>)
+      (h₃ : <{ ~Γ ⊢ ~t₃ ⦂ ~τ₀ }>) :
+      <{ ~Γ ⊢ if0 ~t₁ then ~t₂ else ~t₃ ⦂ ~τ₀ }>
 -- END SOLUTION
 ```
 
@@ -2206,7 +2206,7 @@ partial def unexpandCtx : Term → UnexpandM (TSyntax `stlcCtx)
           `(stlcVar| $(mkIdent (Name.mkSimple x.getString)):ident)
         else `(stlcVar| ~$x)
       match τ with
-      | `(<{ $T':stlcTy }>) => `(stlcCtx| $x':stlcVar ↦ $T' ; $G')
+      | `(<{ $τ':stlcTy }>) => `(stlcCtx| $x':stlcVar ↦ $τ' ; $G')
       | _                   => `(stlcCtx| $x':stlcVar ↦ ~($τ) ; $G')
   | G => `(stlcCtx| ~($G))
 
@@ -2230,8 +2230,8 @@ An example:
 ```lean
 theorem Nat_typing_example : <{ ∅ ⊢ (λ x : Nat . λ y : Nat . x * y) 3 2 ⦂ Nat }> := by
   solution!
-    apply HasType.app (T₂ := Ty.nat)
-    · apply HasType.app (T₂ := Ty.nat)
+    apply HasType.app (τ₂ := Ty.nat)
+    · apply HasType.app (τ₂ := Ty.nat)
       · apply HasType.abs
         apply HasType.abs
         apply HasType.mult
@@ -2260,9 +2260,9 @@ The next lemmas are proved _exactly_ as before.
 :::::exercise (rating := 4) (name := "StlcArith.weakening")
 ```lean
 theorem weakening (Γ Γ' : Context) (t : Tm) (τ : Ty)
-    (hi : Γ ⊆ Γ') (hT : <{ ~Γ ⊢ ~t ⦂ ~τ }>) : <{ ~Γ' ⊢ ~t ⦂ ~τ }> := by
+    (hi : Γ ⊆ Γ') (hτ : <{ ~Γ ⊢ ~t ⦂ ~τ }>) : <{ ~Γ' ⊢ ~t ⦂ ~τ }> := by
   solution!
-    induction hT generalizing Γ' with
+    induction hτ generalizing Γ' with
     | var _ x _ h =>
       constructor
       exact hi h
@@ -2310,29 +2310,29 @@ for the STLC.
 
 ```lean
 -- SOLUTION
-theorem weakening_empty (Γ : Context) (t : Tm) (τ : Ty) (hT : <{ ∅ ⊢ ~t ⦂ ~τ }>) :
+theorem weakening_empty (Γ : Context) (t : Tm) (τ : Ty) (hτ : <{ ∅ ⊢ ~t ⦂ ~τ }>) :
     <{ ~Γ ⊢ ~t ⦂ ~τ }> := by
   apply weakening ∅
   · intros x b contra
     contradiction
   · assumption
 
-theorem substitution_preserves_typing (Γ : Context) (x : String) (U : Ty)
+theorem substitution_preserves_typing (Γ : Context) (x : String) (τ' : Ty)
     (t v : Tm) (τ : Ty)
-    (hT : <{ ~x ↦ ~U ; ~Γ ⊢ ~t ⦂ ~τ }>) (hv : <{ ∅ ⊢ ~v ⦂ ~U }>) :
+    (hτ : <{ ~x ↦ ~τ' ; ~Γ ⊢ ~t ⦂ ~τ }>) (hv : <{ ∅ ⊢ ~v ⦂ ~τ' }>) :
     <{ ~Γ ⊢ [~x := ~v] ~t ⦂ ~τ }> := by
   induction t generalizing Γ τ with
   | var y =>
-    cases hT with
+    cases hτ with
     | var _ _ _ h =>
       by_cases hxy : x = y
       · subst hxy
         rw [PartialMap.update_eq] at h
         rw [subst_var_eq]
-        have hUT : U = τ := by
+        have hτ'τ : τ' = τ := by
           apply Option.some.inj
           exact h
-        subst hUT
+        subst hτ'τ
         apply weakening_empty
         exact hv
       · rw [PartialMap.update_neq hxy] at h
@@ -2340,7 +2340,7 @@ theorem substitution_preserves_typing (Γ : Context) (x : String) (U : Ty)
         constructor
         exact h
   | app t₁ t₂ ih₁ ih₂ =>
-    cases hT with
+    cases hτ with
     | app _ _ _ _ _ h₁ h₂ =>
       rw [subst_app]
       constructor
@@ -2349,7 +2349,7 @@ theorem substitution_preserves_typing (Γ : Context) (x : String) (U : Ty)
       · apply ih₂
         exact h₂
   | abs y S t₁ ih =>
-    cases hT with
+    cases hτ with
     | abs _ _ _ _ _ h =>
       by_cases hxy : x = y
       · subst hxy
@@ -2363,26 +2363,26 @@ theorem substitution_preserves_typing (Γ : Context) (x : String) (U : Ty)
         apply ih
         exact h
   | const n =>
-    cases hT with
+    cases hτ with
     | const =>
       rw [subst_const]
       constructor
   | succ t₁ ih =>
-    cases hT with
+    cases hτ with
     | succ _ _ h =>
       rw [subst_succ]
       constructor
       apply ih
       exact h
   | pred t₁ ih =>
-    cases hT with
+    cases hτ with
     | pred _ _ h =>
       rw [subst_pred]
       constructor
       apply ih
       exact h
   | mult t₁ t₂ ih₁ ih₂ =>
-    cases hT with
+    cases hτ with
     | mult _ _ _ h₁ h₂ =>
       rw [subst_mult]
       constructor
@@ -2391,7 +2391,7 @@ theorem substitution_preserves_typing (Γ : Context) (x : String) (U : Ty)
       · apply ih₂
         exact h₂
   | ite0 t₁ t₂ t₃ ih₁ ih₂ ih₃ =>
-    cases hT with
+    cases hτ with
     | ite0 _ _ _ _ _ h₁ h₂ h₃ =>
       rw [subst_ite0]
       constructor
@@ -2419,14 +2419,14 @@ before.
 
 ```lean
 theorem preservation (t t' : Tm) (τ : Ty)
-    (hT : <{ ∅ ⊢ ~t ⦂ ~τ }>) (hs : t ⟶ t') : <{ ∅ ⊢ ~t' ⦂ ~τ }> := by
+    (hτ : <{ ∅ ⊢ ~t ⦂ ~τ }>) (hs : t ⟶ t') : <{ ∅ ⊢ ~t' ⦂ ~τ }> := by
   solution!
-    generalize hΓ : (∅ : Context) = Γ at hT
-    induction hT generalizing t' with
+    generalize hΓ : (∅ : Context) = Γ at hτ
+    induction hτ generalizing t' with
     | var => cases hs
     | abs => cases hs
     | const => cases hs
-    | app Γ T₁ T₂ t₁ t₂ h₁ h₂ ih₁ ih₂ =>
+    | app Γ τ₁ τ₂ t₁ t₂ h₁ h₂ ih₁ ih₂ =>
       subst hΓ
       cases hs with
       | appAbs _ _ _ _ _ =>
@@ -2482,7 +2482,7 @@ theorem preservation (t t' : Tm) (τ : Ty)
         · apply ih₂
           · exact hst
           · rfl
-    | ite0 Γ t₁ t₂ t₃ T₀ h₁ h₂ h₃ ih₁ ih₂ ih₃ =>
+    | ite0 Γ t₁ t₂ t₃ τ₀ h₁ h₂ h₃ ih₁ ih₂ ih₃ =>
       subst hΓ
       cases hs with
       | if0Step _ t₁' _ _ hst =>
@@ -2510,12 +2510,12 @@ theorem preservation (t t' : Tm) (τ : Ty)
 
 :::::exercise (rating := 4) (name := "StlcArith.progress")
 ```lean
-theorem progress (t : Tm) (τ : Ty) (hT : <{ ∅ ⊢ ~t ⦂ ~τ }>) :
+theorem progress (t : Tm) (τ : Ty) (hτ : <{ ∅ ⊢ ~t ⦂ ~τ }>) :
     t.IsValue ∨ ∃ t', t ⟶ t' := by
   solution!
-    generalize hΓ : (∅ : Context) = Γ at hT
-    induction hT with
-    | var Γ x T₁ h =>
+    generalize hΓ : (∅ : Context) = Γ at hτ
+    induction hτ with
+    | var Γ x τ₁ h =>
       subst hΓ
       -- Contradictory: variables cannot be typed in an empty context.
       rw [PartialMap.getElem_empty] at h
@@ -2526,7 +2526,7 @@ theorem progress (t : Tm) (τ : Ty) (hT : <{ ∅ ⊢ ~t ⦂ ~τ }>) :
     | const _ n =>
       left
       constructor
-    | app Γ T₁ T₂ t₁ t₂ h₁ h₂ ih₁ ih₂ =>
+    | app Γ τ₁ τ₂ t₁ t₂ h₁ h₂ ih₁ ih₂ =>
       right
       subst hΓ
       cases ih₁ rfl with
@@ -2603,7 +2603,7 @@ theorem progress (t : Tm) (τ : Ty) (hT : <{ ∅ ⊢ ~t ⦂ ~τ }>) :
         exists <{ ~t₁' * ~t₂ }>
         apply Step.mult1
         assumption
-    | ite0 Γ t₁ t₂ t₃ T₀ h₁ h₂ h₃ ih₁ ih₂ ih₃ =>
+    | ite0 Γ t₁ t₂ t₃ τ₀ h₁ h₂ h₃ ih₁ ih₂ ih₃ =>
       right
       subst hΓ
       cases ih₁ rfl with
